More extensions to LibFinmap.

LambdaS5/coq/LibFinmap.v
@@ -79,6 +79,19 @@ Class Binds_single_bind_diff_eq `{BagBinds A B T} `{BagSingleBind A B T} :=
 Class Binds_single_bind_diff `{BagBinds A B T} `{BagSingleBind A B T} :=
     { binds_single_bind_diff : forall k k' x x', k <> k' -> ~binds (k' \:= x') k x }.
 
+(* union *)
+Class Binds_union_eq `{BagBinds A B T} `{BagIndex T A} `{BagUnion T} :=
+    { binds_union_eq : forall M1 M2 k x, binds (M1 \u M2) k x = (binds M1 k x \/ ~index M1 k /\ binds M2 k x) }.
+
+Class Binds_union_l `{BagBinds A B T} `{BagUnion T} :=
+    { binds_union_l : forall M1 M2 k x, binds M1 k x -> binds (M1 \u M2) k x }.
+
+Class Binds_union_r `{BagBinds A B T} `{BagIndex T A} `{BagUnion T} :=
+    { binds_union_r : forall M1 M2 k x, ~index M1 k -> binds M2 k x -> binds (M1 \u M2) k x }.
+
+Class Binds_union_inv `{BagBinds A B T} `{BagIndex T A} `{BagUnion T} :=
+    { binds_union_inv : forall M1 M2 k x, binds (M1 \u M2) k x -> binds M1 k x \/ ~index M1 k /\ binds M2 k x }.
+
 (* remove *)
 Class Binds_remove_eq `{BagBinds A B T} `{BagIn A T1} `{BagRemove T T1} :=
     { binds_remove_eq : forall M S k x, binds (M \- S) k x = (binds M k x /\ k \notin S) }.
@@ -178,6 +191,19 @@ Class Index_single_bind_diff_eq `{BagIndex T A} `{BagSingleBind A B T} :=
 
 Class Index_single_bind_diff `{BagIndex T A} `{BagSingleBind A B T} :=
     { index_single_bind_diff : forall k k' x', k <> k' -> ~index (k' \:= x') k }. 
+
+(* union *)
+Class Index_union_eq `{BagIndex T A} `{BagUnion T} :=
+    { index_union_eq : forall M1 M2 k, index (M1 \u M2) k = (index M1 k \/ index M2 k) }.
+
+Class Index_union_l `{BagIndex T A} `{BagUnion T} :=
+    { index_union_l : forall M1 M2 k, index M1 k -> index (M1 \u M2) k }.
+
+Class Index_union_r `{BagIndex T A} `{BagUnion T} :=
+    { index_union_r : forall M1 M2 k, index M2 k -> index (M1 \u M2) k }.
+
+Class Index_union_inv `{BagIndex T A} `{BagUnion T} :=
+    { index_union_inv : forall M1 M2 k, index (M1 \u M2) k -> index M1 k \/ index M2 k }.
 
 (* remove *)
 Class Index_remove_eq `{BagIndex T A} `{BagIn A T1} `{BagRemove T T1} :=
@@ -312,13 +338,21 @@ Instance read_option_binds_inv_from_read_option_binds_eq :
     Read_option_binds_eq -> Read_option_binds_inv.
 Proof. constructor. introv I. rewrite read_option_binds_eq. assumption. Qed.
 
+(* empty *)
+Section BindsEmpty.
+Context `{BagBinds A B T} `{BagEmpty T}.
+
 Instance binds_empty_from_binds_empty_eq :
-    forall `{BagBinds A B T} `{BagEmpty T},
     Binds_empty_eq -> Binds_empty.
 Proof. constructor. introv. rewrite binds_empty_eq. auto. Qed.
 
+End BindsEmpty.
+
+(* single_bind *)
+Section BindsSingleBind.
+Context `{BagBinds A B T} `{BagSingleBind A B T}.
+
 Instance binds_single_bind_same_eq_from_binds_single_bind_eq :
-    forall `{BagBinds A B T} `{BagSingleBind A B T},
     Binds_single_bind_eq -> Binds_single_bind_same_eq. 
 Proof. 
     constructor. intros. rewrite binds_single_bind_eq. rew_logic. 
@@ -326,17 +360,14 @@ Proof.
 Qed.
 
 Instance binds_single_bind_same_from_binds_single_bind_same_eq :
-    forall `{BagBinds A B T} `{BagSingleBind A B T},
     Binds_single_bind_same_eq -> Binds_single_bind_same. 
 Proof. constructor. intros. rewrite binds_single_bind_same_eq. reflexivity. Qed.
 
 Instance binds_single_bind_same_inv_from_binds_single_bind_same_eq :
-    forall `{BagBinds A B T} `{BagSingleBind A B T},
     Binds_single_bind_same_eq -> Binds_single_bind_same_inv. 
 Proof. constructor. introv I. rewrite binds_single_bind_same_eq in I. assumption. Qed.
 
 Instance binds_single_bind_diff_eq_from_binds_single_bind_eq :
-    forall `{BagBinds A B T} `{BagSingleBind A B T},
     Binds_single_bind_eq -> Binds_single_bind_diff_eq. 
 Proof. 
     constructor. intros. rewrite binds_single_bind_eq. rew_logic. 
@@ -344,83 +375,102 @@ Proof.
 Qed.
 
 Instance binds_single_bind_diff_from_binds_single_bind_diff_eq :
-    forall `{BagBinds A B T} `{BagSingleBind A B T},
     Binds_single_bind_diff_eq -> Binds_single_bind_diff. 
 Proof. constructor. introv Hd. rewrite binds_single_bind_diff_eq; auto. Qed.
 
+End BindsSingleBind.
+
+(* union *)
+Section BindsUnion.
+Context `{BagBinds A B T} `{BagIndex T A} `{BagUnion T}.
+
+Instance binds_union_l_from_binds_union_eq :
+    Binds_union_eq -> Binds_union_l.
+Proof. constructor. introv. rewrite binds_union_eq. auto. Qed.
+
+Instance binds_union_r_from_binds_union_eq :
+    Binds_union_eq -> Binds_union_r.
+Proof. constructor. introv. rewrite binds_union_eq. auto. Qed.
+
+Instance binds_union_inv_from_binds_union_eq :
+    Binds_union_eq -> Binds_union_inv.
+Proof. constructor. introv. rewrite binds_union_eq. auto. Qed.
+
+End BindsUnion.
+
 (* remove *)
+Section BindsRemove.
+Context `{BagBinds A B T} `{BagIn A T1} `{BagRemove T T1}.
+
 Instance binds_remove_notin_eq_from_binds_remove_eq :
-    forall `{BagBinds A B T} `{BagIn A T1} `{BagRemove T T1},
     Binds_remove_eq -> Binds_remove_notin_eq.
 Proof. constructor. introv Hin. rewrite binds_remove_eq. rew_logic. 
     apply iff_intro; iauto.
 Qed.
 
 Instance binds_remove_notin_from_binds_remove_notin_eq :
-    forall `{BagBinds A B T} `{BagIn A T1} `{BagRemove T T1},
     Binds_remove_notin_eq -> Binds_remove_notin.
 Proof. constructor. introv Hin I. rewrite binds_remove_notin_eq; auto. Qed.
 
 Instance binds_remove_notin_inv_from_binds_remove_notin_eq :
-    forall `{BagBinds A B T} `{BagIn A T1} `{BagRemove T T1},
     Binds_remove_notin_eq -> Binds_remove_notin_inv.
 Proof. constructor. introv Hin I. rewrite binds_remove_notin_eq in I; auto. Qed.
 
 Instance binds_remove_in_eq_from_binds_remove_eq :
-    forall `{BagBinds A B T} `{BagIn A T1} `{BagRemove T T1},
     Binds_remove_eq -> Binds_remove_in_eq.
 Proof. constructor. introv Hin. rewrite binds_remove_eq. rew_logic. 
     apply iff_intro; iauto.
 Qed.
 
 Instance binds_remove_in_from_binds_remove_in_eq :
-    forall `{BagBinds A B T} `{BagIn A T1} `{BagRemove T T1},
     Binds_remove_in_eq -> Binds_remove_in.
 Proof. constructor. introv Hin.  rewrite binds_remove_in_eq; auto. Qed.
 
 Instance binds_remove_inv_from_binds_remove_eq :
-    forall `{BagBinds A B T} `{BagIn A T1} `{BagRemove T T1},
     Binds_remove_eq -> Binds_remove_inv.
 Proof. constructor. introv Hb. rewrite binds_remove_eq in Hb. auto. Qed.
 
+End BindsRemove.
+
 (* restrict *)
+Section BindsRestrict.
+Context `{BagBinds A B T} `{BagIn A T1} `{BagRestrict T T1}.
+
 Instance binds_restrict_in_eq_from_binds_restrict_eq :
-    forall `{BagBinds A B T} `{BagIn A T1} `{BagRestrict T T1},
     Binds_restrict_eq -> Binds_restrict_in_eq.
 Proof. constructor. introv Hin. rewrite binds_restrict_eq. rew_logic. 
     apply iff_intro; iauto.
 Qed.
 
 Instance binds_restrict_in_from_binds_restrict_in_eq :
-    forall `{BagBinds A B T} `{BagIn A T1} `{BagRestrict T T1},
     Binds_restrict_in_eq -> Binds_restrict_in.
 Proof. constructor. introv Hin I. rewrite binds_restrict_in_eq; auto. Qed.
 
 Instance binds_restrict_in_inv_from_binds_restrict_in_eq :
-    forall `{BagBinds A B T} `{BagIn A T1} `{BagRestrict T T1},
     Binds_restrict_in_eq -> Binds_restrict_in_inv.
 Proof. constructor. introv Hin I. rewrite binds_restrict_in_eq in I; auto. Qed.
 
 Instance binds_restrict_notin_eq_from_binds_restrict_eq :
-    forall `{BagBinds A B T} `{BagIn A T1} `{BagRestrict T T1},
     Binds_restrict_eq -> Binds_restrict_notin_eq.
 Proof. constructor. introv Hin. rewrite binds_restrict_eq. rew_logic. 
     apply iff_intro; iauto.
 Qed.
 
 Instance binds_restrict_notin_from_binds_restrict_notin_eq :
-    forall `{BagBinds A B T} `{BagIn A T1} `{BagRestrict T T1},
     Binds_restrict_notin_eq -> Binds_restrict_notin.
 Proof. constructor. introv Hin.  rewrite binds_restrict_notin_eq; auto. Qed.
 
 Instance binds_restrict_inv_from_binds_restrict_eq :
-    forall `{BagBinds A B T} `{BagIn A T1} `{BagRestrict T T1},
     Binds_restrict_eq -> Binds_restrict_inv.
 Proof. constructor. introv Hb. rewrite binds_restrict_eq in Hb. auto. Qed.
 
+End BindsRestrict.
+
 (* update *)
+Section BindsUpdate.
+Context `{BagBinds A B T} `{BagUpdate A B T}.
+
 Instance binds_update_same_eq_from_binds_update_eq :
-    forall `{BagBinds A B T} `{BagUpdate A B T},
     Binds_update_eq -> Binds_update_same_eq.
 Proof. 
     constructor. intros. rewrite binds_update_eq. rew_logic. 
@@ -428,17 +478,14 @@ Proof.
 Qed.
 
 Instance binds_update_same_from_binds_update_same_eq :
-    forall `{BagBinds A B T} `{BagUpdate A B T},
     Binds_update_same_eq -> Binds_update_same.
 Proof. constructor. intros. rewrite binds_update_same_eq. reflexivity. Qed.
 
 Instance binds_update_same_inv_from_binds_update_same_eq :
-    forall `{BagBinds A B T} `{BagUpdate A B T},
     Binds_update_same_eq -> Binds_update_same_inv.
 Proof. constructor. introv I. rewrite binds_update_same_eq in I. assumption. Qed.
 
 Instance binds_update_diff_eq_from_binds_update_eq :
-    forall `{BagBinds A B T} `{BagUpdate A B T},
     Binds_update_eq -> Binds_update_diff_eq.
 Proof. 
     constructor. intros. rewrite binds_update_eq. rew_logic. 
@@ -446,55 +493,84 @@ Proof.
 Qed.
 
 Instance binds_update_diff_from_binds_update_diff_eq :
-    forall `{BagBinds A B T} `{BagUpdate A B T},
     Binds_update_diff_eq -> Binds_update_diff.
 Proof. constructor. intros. rewrite binds_update_diff_eq; assumption. Qed.
 
 Instance binds_update_diff_inv_from_binds_update_diff_eq :
-    forall `{BagBinds A B T} `{BagUpdate A B T},
     Binds_update_diff_eq -> Binds_update_diff_inv.
 Proof. constructor. introv Hd I. rewrite binds_update_diff_eq in I; assumption. Qed.
 
+End BindsUpdate.
+
+(* index binds *)
+Section IndexBinds.
+Context `{BagIndex T A} `{BagBinds A B T}.
+
 Instance index_binds_from_index_binds_eq :
-    forall `{BagIndex T A} `{BagBinds A B T},
     Index_binds_eq -> Index_binds.
 Proof. constructor. introv I. rewrite index_binds_eq in I. assumption. Qed.
 
 Instance index_binds_inv_from_index_binds_eq :
-    forall `{BagIndex T A} `{BagBinds A B T},
     Index_binds_eq -> Index_binds_inv.
 Proof. constructor. introv I. rewrite index_binds_eq. eauto. Qed.
 
+End IndexBinds.
+
 (* empty *)
+Section IndexEmpty.
+Context `{BagIndex T A} `{BagEmpty T}.
+
 Instance index_empty_from_index_empty_eq :
-    forall `{BagIndex T A} `{BagEmpty T},
     Index_empty_eq -> Index_empty.
 Proof. constructor. introv. rewrite index_empty_eq. auto. Qed. 
 
+End IndexEmpty.
+
 (* single_bind *)
+Section IndexSingleBind.
+Context `{BagIndex T A} `{BagSingleBind A B T}.
+
 Instance index_single_bind_same_eq_from_index_single_bind_eq :
-    forall `{BagIndex T A} `{BagSingleBind A B T},
     Index_single_bind_eq -> Index_single_bind_same_eq.
 Proof. constructor. introv. rewrite index_single_bind_eq. auto. Qed.
 
 Instance index_single_bind_same_from_index_single_bind_same_eq :
-    forall `{BagIndex T A} `{BagSingleBind A B T},
     Index_single_bind_same_eq -> Index_single_bind_same.
 Proof. constructor. introv. rewrite index_single_bind_same_eq. auto. Qed.
 
 Instance index_single_bind_diff_eq_from_index_single_bind_eq :
-    forall `{BagIndex T A} `{BagSingleBind A B T},
     Index_single_bind_eq -> Index_single_bind_diff_eq.
 Proof. constructor. introv. rewrite index_single_bind_eq. auto. Qed.
 
 Instance index_single_bind_diff_from_index_single_bind_diff_eq :
-    forall `{BagIndex T A} `{BagSingleBind A B T},
     Index_single_bind_diff_eq -> Index_single_bind_diff.
 Proof. constructor. introv Hd. rewrite index_single_bind_diff_eq; auto. Qed.
 
+End IndexSingleBind.
+
+(* union *)
+Section IndexUnion.
+Context `{BagIndex T A} `{BagUnion T}.
+
+Instance index_union_l_from_index_union_eq :
+    Index_union_eq -> Index_union_l.
+Proof. constructor. introv. rewrite index_union_eq. auto. Qed.
+
+Instance index_union_r_from_index_union_eq :
+    Index_union_eq -> Index_union_inv.
+Proof. constructor. introv. rewrite index_union_eq. auto. Qed.
+
+Instance index_union_inv_from_index_union_eq :
+    Index_union_eq -> Index_union_inv.
+Proof. constructor. introv. rewrite index_union_eq. auto. Qed.
+
+End IndexUnion.
+
 (* remove *)
+Section IndexRemove.
+Context `{BagIndex T A} `{BagIn A T1} `{BagRemove T T1}.
+
 Instance index_remove_in_eq_from_index_remove_eq :
-    forall `{BagIndex T A} `{BagIn A T1} `{BagRemove T T1},
     Index_remove_eq -> Index_remove_in_eq.
 Proof. 
     constructor. introv I. rewrite index_remove_eq. rew_logic. 
@@ -502,12 +578,10 @@ Proof.
 Qed.
 
 Instance index_remove_in_from_index_remove_in_eq :
-    forall `{BagIndex T A} `{BagIn A T1} `{BagRemove T T1},
     Index_remove_in_eq -> Index_remove_in.
 Proof. constructor. introv Hi. rewrite index_remove_in_eq; auto. Qed.
 
 Instance index_remove_notin_eq_from_index_remove_eq :
-    forall `{BagIndex T A} `{BagIn A T1} `{BagRemove T T1},
     Index_remove_eq -> Index_remove_notin_eq.
 Proof. 
     constructor. introv I. rewrite index_remove_eq. rew_logic. 
@@ -515,18 +589,20 @@ Proof.
 Qed.
 
 Instance index_remove_notin_from_index_remove_notin_eq :
-    forall `{BagIndex T A} `{BagIn A T1} `{BagRemove T T1},
     Index_remove_notin_eq -> Index_remove_notin.
 Proof. constructor. introv Hi. rewrite index_remove_notin_eq; auto. Qed.
 
 Instance index_remove_notin_inv_from_index_remove_notin_eq :
-    forall `{BagIndex T A} `{BagIn A T1} `{BagRemove T T1},
     Index_remove_notin_eq -> Index_remove_notin_inv.
 Proof. constructor. introv Hi. rewrite index_remove_notin_eq; auto. Qed.
 
+End IndexRemove.
+
 (* restrict *)
+Section IndexRestrict.
+Context `{BagIndex T A} `{BagIn A T1} `{BagRestrict T T1}.
+
 Instance index_restrict_notin_eq_from_index_restrict_eq :
-    forall `{BagIndex T A} `{BagIn A T1} `{BagRestrict T T1},
     Index_restrict_eq -> Index_restrict_notin_eq.
 Proof. 
     constructor. introv I. rewrite index_restrict_eq. rew_logic. 
@@ -534,12 +610,10 @@ Proof.
 Qed.
 
 Instance index_restrict_notin_from_index_restrict_notin_eq :
-    forall `{BagIndex T A} `{BagIn A T1} `{BagRestrict T T1},
     Index_restrict_notin_eq -> Index_restrict_notin.
 Proof. constructor. introv Hi. rewrite index_restrict_notin_eq; auto. Qed.
 
 Instance index_restrict_in_eq_from_index_restrict_eq :
-    forall `{BagIndex T A} `{BagIn A T1} `{BagRestrict T T1},
     Index_restrict_eq -> Index_restrict_in_eq.
 Proof. 
     constructor. introv I. rewrite index_restrict_eq. rew_logic. 
@@ -547,33 +621,32 @@ Proof.
 Qed.
 
 Instance index_restrict_in_from_index_restrict_in_eq :
-    forall `{BagIndex T A} `{BagIn A T1} `{BagRestrict T T1},
     Index_restrict_in_eq -> Index_restrict_in.
 Proof. constructor. introv Hi. rewrite index_restrict_in_eq; auto. Qed.
 
 Instance index_restrict_in_inv_from_index_restrict_in_eq :
-    forall `{BagIndex T A} `{BagIn A T1} `{BagRestrict T T1},
     Index_restrict_in_eq -> Index_restrict_in_inv.
 Proof. constructor. introv Hi. rewrite index_restrict_in_eq; auto. Qed.
 
+End IndexRestrict.
+
 (* update *)
+Section IndexUpdate.
+Context `{BagIndex T A} `{BagUpdate A B T}.
+
 Instance index_update_same_eq_from_index_update_eq : 
-    forall `{BagIndex T A} `{BagUpdate A B T},
     Index_update_eq -> Index_update_same_eq.
 Proof. constructor. introv. rewrite index_update_eq. auto. Qed.
 
 Instance index_update_same_from_index_update_same_eq :
-    forall `{BagIndex T A} `{BagUpdate A B T},
     Index_update_same_eq -> Index_update_same.
 Proof. constructor. introv. rewrite index_update_same_eq. auto. Qed.
 
 Instance index_update_index_from_index_update_eq : 
-    forall `{BagIndex T A} `{BagUpdate A B T},
     Index_update_eq -> Index_update_index.
 Proof. constructor. introv. rewrite index_update_eq. auto. Qed.
 
 Instance index_update_diff_eq_from_index_update_eq : 
-    forall `{BagIndex T A} `{BagUpdate A B T},
     Index_update_eq -> Index_update_diff_eq.
 Proof. 
     constructor. introv Hd. rewrite index_update_eq. rew_logic.
@@ -581,14 +654,14 @@ Proof.
 Qed.
 
 Instance index_update_diff_from_index_update_diff_eq :
-    forall `{BagIndex T A} `{BagUpdate A B T},
     Index_update_diff_eq -> Index_update_diff.
 Proof. constructor. introv Hd. rewrite index_update_diff_eq; eauto. Qed.
 
 Instance index_update_diff_inv_from_index_update_diff_eq :
-    forall `{BagIndex T A} `{BagUpdate A B T},
     Index_update_diff_eq -> Index_update_diff_inv.
 Proof. constructor. introv Hd. rewrite index_update_diff_eq; auto. Qed.
+
+End IndexUpdate.
 
 Instance fresh_index_from_fresh_index_eq : 
     forall `{BagIndex T A} `{BagFresh A T}, 
@@ -630,13 +703,17 @@ Qed.
 
 Create HintDb bag discriminated.
 
-Hint Resolve @binds_empty @binds_single_bind_same @binds_single_bind_diff
+Hint Resolve 
+    @binds_empty @binds_single_bind_same @binds_single_bind_diff
+    @binds_union_l @binds_union_r
     @binds_remove_in @binds_remove_notin
     @binds_restrict_in @binds_restrict_notin
     @binds_update_same @binds_update_diff 
     @index_binds_inv @fresh_index 
     @incl_binds @update_nindex_incl 
+    @remove_incl @restrict_incl
     @index_empty @index_single_bind_same @index_single_bind_diff
+    @index_union_l @index_union_r
     @index_remove_in @index_remove_notin
     @index_restrict_in @index_restrict_notin
     @index_update_same @index_update_index @index_update_diff
@@ -645,9 +722,10 @@ Hint Resolve @binds_empty @binds_single_bind_same @binds_single_bind_diff
 Tactic Notation "prove_bag" :=
     solve [ eauto with bag typeclass_instances ].
 
-(* TODO why doesn't this work?
-Hint Rewrite @binds_empty_eq @binds_single_bind_eq @binds_remove_eq 
-    @binds_update_eq @incl_binds_eq @index_binds_eq : rew_binds_eq.
+Hint Rewrite @binds_empty_eq @binds_single_bind_eq @binds_union_eq
+    @binds_remove_eq @binds_restrict_eq
+    @binds_update_eq @incl_binds_eq @index_binds_eq  
+    using (eauto with typeclass_instances) : rew_binds_eq.
 
 Tactic Notation "rew_binds_eq" :=
     autorewrite with rew_binds_eq.
@@ -664,19 +742,18 @@ Tactic Notation "rew_binds_eq" "~" "in" hyp(H) :=
     rew_binds_eq in H; auto_tilde.
 Tactic Notation "rew_binds_eq" "*" "in" hyp(H) :=
     rew_binds_eq in H; auto_star.
-*)
 
 Instance update_nindex_incl_inst :
     forall `{BagIncl T} `{BagUpdate A B T} `{BagIndex T A} `{BagBinds A B T},
     Index_binds_eq -> Incl_binds_eq -> Binds_update_eq -> Update_nindex_incl.
 Proof.
-    constructor. introv. 
+    constructor. introv.
     rewrite incl_binds_eq, index_binds_eq. 
-    rew_logic. intros.
-    rewrite binds_update_eq. 
+    rew_logic. intros. 
+    rew_binds_eq.
     right. split.
     intro. substs. jauto.
-    auto.
+    auto. 
 Qed.
 
 Instance remove_incl_inst :
@@ -684,7 +761,7 @@ Instance remove_incl_inst :
     Binds_remove_eq -> Incl_binds_eq -> Remove_incl.
 Proof.
     constructor. introv.
-    rewrite incl_binds_eq. introv.
+    rewrite incl_binds_eq. introv. 
     rewrite binds_remove_eq.
     iauto.
 Qed.
@@ -715,7 +792,18 @@ Instance index_single_bind_eq_inst :
 Proof.
     constructor. introv. rewrite index_binds_eq. 
     rew_logic; apply iff_intro; 
-    jauto_set; rewrites binds_single_bind_eq in *; jauto.
+    jauto_set; rew_binds_eq in *; jauto.
+Qed.
+
+Instance index_union_eq_inst :
+    forall `{BagIndex T A} `{BagBinds A B T} `{BagUnion T},
+    Index_binds_eq -> Binds_union_eq -> Index_union_eq.
+Proof.
+    constructor. introv. rewrite_all index_binds_eq.
+    rew_logic; apply iff_intro; introv Hi.
+    jauto_set; rewrites binds_union_eq in *; iauto.
+    apply case_classic_l in Hi.
+    destruct Hi; jauto_set; rewrites binds_union_eq; rewrites index_binds_eq; iauto.
 Qed.
 
 Instance index_remove_eq_inst :
@@ -725,6 +813,15 @@ Proof.
     constructor. introv. rewrite_all index_binds_eq.
     rew_logic; apply iff_intro; 
     jauto_set; rewrites binds_remove_eq in *; jauto.
+Qed.
+
+Instance index_restrict_eq_inst :
+    forall `{BagIndex T A} `{BagBinds A B T} `{BagIn A T1} `{BagRestrict T T1},
+    Index_binds_eq -> Binds_restrict_eq -> Index_restrict_eq.
+Proof.
+    constructor. introv. rewrite_all index_binds_eq.
+    rew_logic; apply iff_intro; 
+    jauto_set; rewrites binds_restrict_eq in *; jauto.
 Qed.
 
 Instance index_update_eq_inst :
@@ -772,6 +869,7 @@ Parameter binds_impl : finmap A B -> A -> B -> Prop.
 Parameter incl_impl : finmap A B -> finmap A B -> Prop.
 Parameter read_impl : Inhab B -> finmap A B -> A -> B.
 Parameter read_option_impl : finmap A B -> A -> option B.
+Parameter union_impl : finmap A B -> finmap A B -> finmap A B.
 Parameter remove_impl : finmap A B -> finset A -> finmap A B.
 Parameter restrict_impl : finmap A B -> finset A -> finmap A B.
 Parameter update_impl : finmap A B -> A -> B -> finmap A B.
@@ -785,6 +883,8 @@ Parameter read_option_binds_eq_impl : forall M k x, (read_option_impl M k = Some
 Parameter binds_empty_eq_impl : forall k x, binds_impl empty_impl k x = False.
 Parameter binds_single_bind_eq_impl : forall k k' x x', 
     binds_impl (single_bind_impl k' x') k x = (k = k' /\ x = x').
+Parameter binds_union_eq_impl : forall M1 M2 k x,
+    binds_impl (union_impl M1 M2) k x = (binds_impl M1 k x \/ ~index_impl M1 k /\ binds_impl M2 k x).
 Parameter binds_remove_eq_impl : forall M S k x,
     binds_impl (remove_impl M S) k x = (binds_impl M k x /\ k \notin S).
 Parameter binds_restrict_eq_impl : forall M S k x,
@@ -827,6 +927,8 @@ Definition build_finmap `(F:finite U) : finmap := exist finite U F.
 (* TODO: most properties should follow from finset and map properties.
    Nice prerequisite: lib-bag-ize LibMap. *)
 
+Set Implicit Arguments.
+
 Lemma finite_empty : finite \{}.
 Proof.
   exists (\{} : finset A). 
@@ -849,8 +951,6 @@ Proof.
   introv [S1 E1]. exists S1. 
 Admitted.
 
-Set Implicit Arguments.
-
 Lemma update_finite : forall U k x, finite U -> finite (U \(k := x)).
 Proof.
   introv [S1 E1]. exists (S1 \u \{k}).
@@ -863,6 +963,7 @@ Definition binds_impl M k x : Prop := binds (proj1_sig M) k x.
 Definition incl_impl M1 M2 : Prop := forall k x, binds_impl M1 k x -> binds_impl M2 k x.
 Definition read_option_impl M k : option B := proj1_sig M k. (* TODO abstract it!!! change TLC *)
 Definition read_impl M k : B := proj1_sig M \(k).
+Definition union_impl M1 M2 : finmap := build_finmap (union_finite (proj2_sig M1) (proj2_sig M2)).
 Definition remove_impl M (S : finset A) : finmap.
 Admitted.
 Definition restrict_impl M (S : finset A) : finmap.
@@ -897,6 +998,8 @@ Proof. unfold incl_impl. auto. Qed.
 Parameter binds_empty_eq_impl : forall k x, binds_impl empty_impl k x = False.
 Parameter binds_single_bind_eq_impl : forall k k' x x', 
     binds_impl (single_bind_impl k' x') k x = (k = k' /\ x = x').
+Parameter binds_union_eq_impl : forall M1 M2 k x,
+    binds_impl (union_impl M1 M2) k x = (binds_impl M1 k x \/ ~index_impl M1 k /\ binds_impl M2 k x).
 Parameter binds_remove_eq_impl : forall M S k x,
     binds_impl (remove_impl M S) k x = (binds_impl M k x /\ k \notin S).
 Parameter binds_restrict_eq_impl : forall M S k x,
@@ -948,6 +1051,9 @@ Global Instance read_inst : BagRead A B (finmap A B) :=
 Global Instance read_option_inst : BagReadOption A B (finmap A B) :=
     { read_option := @read_option_impl _ _ }.
 
+Global Instance union_inst : BagUnion (finmap A B) :=
+    { union := @union_impl _ _ }.
+
 Global Instance remove_inst : BagRemove (finmap A B) (finset A) :=
     { remove := @remove_impl _ _ }.
 
@@ -983,6 +1089,9 @@ Global Instance binds_empty_eq_inst : Binds_empty_eq :=
 
 Global Instance binds_single_bind_eq_inst : Binds_single_bind_eq := 
     { binds_single_bind_eq := @binds_single_bind_eq_impl _ _ }.
+
+Global Instance binds_union_eq_inst : Binds_union_eq :=
+    { binds_union_eq := @binds_union_eq_impl _ _ }.
 
 Global Instance binds_remove_eq_inst : Binds_remove_eq :=
     { binds_remove_eq := @binds_remove_eq_impl _ _ }.
@@ -1022,7 +1131,7 @@ Extract Constant FinmapImpl.empty_impl => "BatMap.empty".
 Extract Constant FinmapImpl.single_bind_impl => "fun k x -> BatMap.singleton k x".
 Extract Constant FinmapImpl.read_impl => "fun m k -> BatMap.find k m".
 Extract Constant FinmapImpl.read_option_impl => "fun m k -> try Some (BatMap.find k m) with Not_found -> None".
-(* Extract Constant FinmapImpl.remove_impl => "fun m k -> BatMap.remove k m". *)
+Extract Constant FinmapImpl.union_impl => "fun m1 m2 -> BatMap.union m2 m1".
 Extract Constant FinmapImpl.remove_impl => "fun m s -> BatList.fold_right (BatMap.remove) (FinsetImpl.to_list_impl s) m". 
 Extract Constant FinmapImpl.restrict_impl => "fun m s -> BatList.fold_left (fun cc i -> BatMap.add i (BatMap.find i m) cc) BatMap.empty (FinsetImpl.to_list_impl s)".
 Extract Constant FinmapImpl.update_impl => "fun m k x -> BatMap.add k x m".
